src/program_proof/memkv/connman_proof.v
@@ -11,27 +11,137 @@ Section connman_proof.
 Context `{!rpcregG Σ}.
 Context `{hG: !heapGS Σ}.
 Definition connmanN := nroot .@ "connman".
-Definition own_ConnMan (c_ptr:loc) : iProp Σ :=
-  ∃ (mref:loc) (rpcClsV:gmap u64 val) (rpcClsM:gmap u64 loc),
-    "HrpcCls" ∷ c_ptr ↦[ConnMan :: "rpcCls"] #mref ∗
-    "Hcls_map" ∷ map.is_map mref 1 (rpcClsV, zero_val (struct.ptrT rpc.RPCClient)) ∗
-    "#HownRpcCls" ∷ [∗ map] host ↦ cl;v ∈ rpcClsM;rpcClsV, RPCClient_own cl host ∗ ⌜v = #cl⌝
+Definition own_ConnMan (c_ptr:loc) (lock: val) : iProp Σ :=
+  ∃ (rpcCls making:loc) (rpcClsM makingM:gmap u64 loc),
+    "HrpcCls" ∷ c_ptr ↦[ConnMan :: "rpcCls"] #rpcCls ∗
+    "Hmaking" ∷ c_ptr ↦[ConnMan :: "making"] #making ∗
+    "Hcls_map" ∷ is_map rpcCls 1 rpcClsM ∗
+    "Hmaking_map" ∷ is_map making 1 makingM ∗
+    "#HownRpcCls" ∷ ([∗ map] host ↦ cl ∈ rpcClsM, RPCClient_own cl host) ∗
+    "#HownMaking" ∷ ([∗ map] host ↦ c ∈ makingM, is_cond c lock)
 .
 
 Definition is_ConnMan (c_ptr:loc) : iProp Σ :=
   ∃ mu,
   "#Hmu" ∷ readonly (c_ptr ↦[ConnMan :: "mu"] mu) ∗
-  "#Hinv" ∷ is_lock connmanN mu (own_ConnMan c_ptr)
+  "#Hinv" ∷ is_lock connmanN mu (own_ConnMan c_ptr mu)
 .
 
-Lemma wp_ConnMan__Call {X:Type} (x:X) γsmap (c_ptr:loc) (rpcid:u64) (host:u64) req rep_out_ptr
+Local Lemma wp_ConnMan__getClient (c_ptr:loc) (host:u64) :
+  is_ConnMan c_ptr -∗
+  {{{ True }}}
+    ConnMan__getClient #c_ptr #host
+  {{{
+    (cl_ptr:loc), RET #cl_ptr; RPCClient_own cl_ptr host
+  }}}.
+Proof.
+  iIntros "#Hconn !# %Φ _ HΦ".
+  iNamed "Hconn".
+  Opaque rpc.RPCClient.
+  Opaque zero_val.
+  wp_lam. wp_pures.
+  wp_apply (wp_ref_of_zero).
+  { done. }
+  iIntros (cl_ptr) "Hcl_ptr".
+  wp_pures.
+  wp_loadField.
+  wp_apply (acquire_spec with "Hinv").
+  iIntros "[Hlocked Hown]".
+  wp_pures.
+  wp_apply (wp_forBreak' with "[-]").
+  { iNamedAccu. }
+  iIntros "!> H". iNamed "H". wp_pures.
+  iNamed "Hown".
+  (* Inside the loop body *)
+  wp_loadField.
+  wp_apply (wp_MapGet with "Hcls_map").
+  iIntros (cl1 ok1) "[%Hcl1 Hcls_map]".
+  wp_pures.
+  destruct ok1.
+  { apply map_get_true in Hcl1.
+    wp_pures.
+    wp_store.
+    wp_pures.
+    iModIntro. iRight. iSplitR; first done.
+    wp_pures.
+    wp_loadField.
+    wp_apply (release_spec with "[$Hinv $Hlocked HrpcCls Hmaking Hmaking_map Hcls_map]").
+    { rewrite /own_ConnMan. eauto 10 with iFrame. }
+    wp_pures.
+    wp_load.
+    iApply "HΦ".
+    iDestruct (big_sepM_lookup with "HownRpcCls") as "$"; done. }
+  apply map_get_false in Hcl1.
+  wp_pures.
+  wp_loadField.
+  wp_apply (wp_MapGet with "Hmaking_map").
+  iIntros (mk2 ok2) "[%Hmk2 Hmaking_map]".
+  wp_pures.
+  destruct ok2.
+  { apply map_get_true in Hmk2.
+    wp_pures.
+    iDestruct (big_sepM_lookup with "HownMaking") as "Hcond"; first done.
+    wp_apply (wp_condWait with "[$Hinv $Hcond $Hlocked HrpcCls Hmaking Hmaking_map Hcls_map]").
+    { rewrite /own_ConnMan. eauto 10 with iFrame. }
+    iIntros "[Hlocked Hown]".
+    wp_pures.
+    iModIntro. iLeft. iSplitR; first done.
+    iFrame. }
+  apply map_get_false in Hmk2.
+  wp_pures.
+  wp_loadField.
+  wp_apply (wp_newCond with "Hinv").
+  iIntros (cond) "#Hcond".
+  wp_loadField.
+  wp_apply (wp_MapInsert _ _ _ _ cond with "Hmaking_map"); first done.
+  iIntros "Hmaking_map".
+  wp_pures.
+  iDestruct (big_sepM_insert_2 with "[Hcond] HownMaking") as "{HownMaking} #HownMaking".
+  { done. }
+  wp_loadField.
+  wp_apply (release_spec with "[$Hinv $Hlocked HrpcCls Hmaking Hmaking_map Hcls_map]").
+  { rewrite /own_ConnMan. eauto 10 with iFrame. }
+  wp_pures.
+  wp_apply wp_MakeRPCClient.
+  iIntros (cl_new) "#Hcl_new".
+  wp_store.
+  wp_loadField.
+  wp_apply (acquire_spec with "Hinv").
+  iIntros "[Hlocked Hown]".
+  iClear "HownRpcCls HownMaking". clear rpcCls making rpcClsM makingM cl1 mk2 Hcl1 Hmk2.
+  wp_pures.
+  iNamed "Hown".
+  wp_load.
+  wp_loadField.
+  wp_apply (wp_MapInsert _ _ _ _ cl_new with "Hcls_map"); first done.
+  iIntros "Hcls_map".
+  iDestruct (big_sepM_insert_2 with "[Hcl_new] HownRpcCls") as "{HownRpcCls} #HownRpcCls".
+  { done. }
+  wp_pures.
+  wp_apply (wp_condBroadcast with "Hcond").
+  wp_pures.
+  wp_loadField.
+  wp_apply (wp_MapDelete with "Hmaking_map"). iIntros "Hmaking_map".
+  iDestruct (big_sepM_subseteq _ _ (map_del makingM host) with "HownMaking") as "{HownMaking} HownMaking".
+  { apply: delete_subseteq. }
+  wp_pures.
+  iModIntro. iRight. iSplitR; first done.
+  wp_pures.
+  wp_loadField.
+  wp_apply (release_spec with "[$Hinv $Hlocked HrpcCls Hmaking Hmaking_map Hcls_map]").
+  { rewrite /own_ConnMan. eauto 10 with iFrame. }
+  wp_load.
+  iApply "HΦ". done.
+Qed.
+
+Lemma wp_ConnMan__CallAtLeastOnce {X:Type} (x:X) γsmap (c_ptr:loc) (rpcid:u64) (host:u64) req rep_out_ptr
       (timeout_ms : u64) dummy_sl_val (reqData:list u8) Pre Post :
   is_ConnMan c_ptr -∗
+  handler_is γsmap X host rpcid Pre Post -∗
+  □(▷ Pre x reqData) -∗
   {{{
       is_slice req byteT 1 reqData ∗
-      rep_out_ptr ↦[slice.T byteT] dummy_sl_val ∗
-      handler_is γsmap X host rpcid Pre Post ∗
-      □(▷ Pre x reqData)
+      rep_out_ptr ↦[slice.T byteT] dummy_sl_val
   }}}
       ConnMan__CallAtLeastOnce #c_ptr #host #rpcid (slice_val req) #rep_out_ptr #timeout_ms
     {{{
@@ -44,9 +154,8 @@ Lemma wp_ConnMan__Call {X:Type} (x:X) γsmap (c_ptr:loc) (rpcid:u64) (host:u64) 
     }}}
     .
 Proof.
-  iIntros "#Hconn !#" (Φ) "Hpre HΦ".
-  iDestruct "Hpre" as "(Hslice & Hrep & #Hhandler & #Hpre)".
-  iNamed "Hconn".
+  iIntros "#Hconn #Hhandler #Hpre !#" (Φ) "H HΦ".
+  iDestruct "H" as "(Hslice & Hrep)".
   Opaque rpc.RPCClient.
   Opaque zero_val.
   wp_lam.
@@ -55,61 +164,23 @@ Proof.
   { done. }
   iIntros (cl_ptr) "Hcl_ptr".
   wp_pures.
-  wp_loadField.
-  wp_apply (acquire_spec with "Hinv").
-  iIntros "[Hlocked Hown]".
-  iNamed "Hown".
+  wp_apply (wp_ConnMan__getClient with "Hconn").
+  iIntros (cl) "Hcl".
+  wp_store.
+  iAssert (∃ cl : loc, cl_ptr ↦[refT (struct.t rpc.RPCClient)] #cl ∗ RPCClient_own cl host)%I with "[Hcl Hcl_ptr]" as "Hcl".
+  { eauto with iFrame. }
+  clear cl.
   wp_pures.
-  wp_loadField.
-  wp_apply (map.wp_MapGet with "Hcls_map").
-  iIntros (cl1 ok1) "[%Hcl1 Hcls_map]".
-  wp_pures.
-  wp_apply (wp_If_join (∃ (cl:loc), "Hown" ∷ own_ConnMan c_ptr ∗
-                        "Hcl" ∷ cl_ptr ↦[refT (struct.t rpc.RPCClient)] #cl ∗
-                        "#HisRpcCl" ∷ RPCClient_own cl host ∗
-                        "Hlocked" ∷ locked mu
-                       ) with "[-Hslice Hrep Hpre HΦ]"); first iSplit.
-  { (* *)
-    iIntros "HΦ".
-    (* TODO: apply spec for getNewClient *)
-    admit.
-  }
-  {
-    iIntros "[%Hnegb HΦ]".
-
-    destruct ok1 as [|] eqn:Hok; last first.
-    { exfalso. done. }
-    apply map.map_get_true in Hcl1.
-    iDestruct (big_sepM2_lookup_r with "HownRpcCls") as "HH".
-    { done. }
-    iDestruct "HH" as (cl) "[%Hcl [#HrpcCl %HclVal]]".
-
-    wp_apply (wp_StoreAt with "Hcl_ptr").
-    { naive_solver. }
-    iIntros "Hcl_ptr".
-    iApply "HΦ".
-
-    iExists cl.
-    rewrite HclVal.
-    iFrame "Hcl_ptr Hlocked #".
-    iExists _,_,_.
-    iFrame "∗#".
-  }
-  iNamed 1.
-  wp_pures.
-  wp_loadField.
-  wp_apply (release_spec with "[$Hinv $Hlocked $Hown]").
-  wp_pures.
-  wp_forBreak_cond.
-  wp_pures.
+  wp_apply (wp_forBreak' with "[-]").
+  { iNamedAccu. }
+  iIntros "!> H". iNamed "H". wp_pures.
+  (* Inside loop body *)
+  iPoseProof "Hconn" as "Hconn2".
+  iNamed "Hconn2".
+  iDestruct "Hcl" as (cl) "[Hcl_ptr #Hcl]".
   wp_load.
-  wp_apply (wp_RPCClient__Call with "[$Hslice $Hrep $Hhandler $HisRpcCl Hpre]").
-  {
-    instantiate (1:=x).
-    iModIntro.
-    iModIntro.
-    done.
-  }
+  wp_apply (wp_RPCClient__Call with "[$Hslice $Hrep $Hhandler $Hcl Hpre]").
+  { done. }
   iIntros (err).
   iIntros "(_ & Hslice & Hrep)".
   wp_pures.
@@ -121,40 +192,57 @@ Proof.
       wp_pures.
       iModIntro.
       iLeft.
-      iSplitL ""; first done.
-      iFrame.
+      iSplitR; first done.
+      eauto with iFrame.
     }
     { (* ErrDisconnected *)
       wp_pures.
       wp_loadField.
       wp_apply (acquire_spec with "Hinv").
       iIntros "[Hlocked Hown]".
-      iClear "HownRpcCls".
+      iClear "Hcl".
       iNamed "Hown".
       wp_pures.
       wp_load.
       wp_loadField.
-      wp_apply (map.wp_MapGet with "Hcls_map").
+      wp_apply (wp_MapGet with "Hcls_map").
       iIntros (cl2 ok2) "[%Hcl2 Hcls_map]".
-      wp_apply (wp_If_join (∃ (cl:loc), "Hown" ∷ own_ConnMan c_ptr ∗
-                                               "Hcl" ∷ cl_ptr ↦[refT (struct.t rpc.RPCClient)] #cl ∗
-                                               "#HisRpcCl" ∷ RPCClient_own cl host ∗
-                                               "Hlocked" ∷ locked mu
-                           ) with "[-Hslice Hrep Hpre HΦ]"); first iSplit.
-      {
-        iIntros "[%Hnegb HΦ]".
-        wp_loadField.
-        wp_apply (map.wp_MapGet with "Hcls_map").
-        iIntros (cl3 ok3) "[%Hcl3 Hcls_map]".
-        wp_pures.
-        admit.
-      }
-      {
-        admit.
-      }
-      admit.
+      wp_apply (wp_If_join_evar with "[HrpcCls Hcls_map]").
+      { iIntros (succ Hsucc).
+        case_bool_decide as Heq; wp_pures.
+        - wp_loadField.
+          wp_apply (wp_MapDelete with "Hcls_map").
+          iIntros "Hcls_map".
+          wp_pures. iModIntro. iSplitR; first done.
+          replace (map_del rpcClsM host) with
+            (if succ then (map_del rpcClsM host) else rpcClsM); last by rewrite Hsucc.
+          iNamedAccu.
+        - iModIntro. iSplitR; first done.
+          rewrite Hsucc. iFrame. }
+      iIntros "H". iNamed "H". wp_pures.
+      wp_loadField.
+      wp_apply (release_spec with "[$Hinv $Hlocked HrpcCls Hmaking Hmaking_map Hcls_map]").
+      { rewrite /own_ConnMan. iModIntro. do 4 iExists _. iFrame. iFrame "HownMaking".
+        case_bool_decide as Heq.
+        - iDestruct (big_sepM_subseteq with "HownRpcCls") as "$".
+          { apply: delete_subseteq. }
+        - iFrame "#". }
+      wp_pures.
+      iClear "HownRpcCls HownMaking". clear rpcCls making rpcClsM makingM Hcl2.
+      wp_apply (wp_ConnMan__getClient with "Hconn").
+      iIntros (cl') "#Hcl'".
+      wp_store.
+      wp_pures.
+      iModIntro. iLeft. iSplitR; first done.
+      eauto with iFrame.
     }
-  }
-Admitted.
+  } 
+  (* no err *)
+  wp_pures.
+  iModIntro. iRight. iSplitR; first done.
+  iApply "HΦ".
+  iDestruct "Hrep" as (rep_sl repData) "(? & ? & ?)".
+  eauto with iFrame.
+Qed.
 
 End connman_proof.
